steel/dist/krmlinit.c
@@ -12,6 +12,7 @@ __attribute__ ((visibility ("hidden")))
 
 void krmlinit_globals()
 {
+  Zeta_Steel_AEADHandle_aead_handle = Zeta_Steel_AEADHandle_init_aead_handle();
   Zeta_Steel_Main_top_level_state *r2_state = Zeta_Steel_Main_init();
   Zeta_Steel_SafeMain_Handle_handle = r2_state;
 }
