steel/crypto/EverCrypt.AEAD.fsti
@@ -1,6 +1,7 @@
 module EverCrypt.AEAD
 open Steel.ST.Util
-module R = Steel.Reference
+module StRef = Steel.ST.Reference
+module NullableRef = Steel.Reference
 module A = Steel.ST.Array
 module U32 = FStar.UInt32
 module S = FStar.SizeT
@@ -35,6 +36,123 @@ val spec (k_bytes:lbytes key_size)
   : GTot (lbytes tag_size)
 
 
+
+
+// /**
+// Create the required AEAD state for the algorithm.
+
+// Note: The caller must free the AEAD state by calling `EverCrypt_AEAD_free`.
+
+// @param a The argument `a` must be either of:
+//   * `Spec_Agile_AEAD_AES128_GCM` (KEY_LEN=16),
+//   * `Spec_Agile_AEAD_AES256_GCM` (KEY_LEN=32), or
+//   * `Spec_Agile_AEAD_CHACHA20_POLY1305` (KEY_LEN=32).
+// @param dst Pointer to a pointer where the address of the allocated AEAD state will be written to.
+// @param k Pointer to `KEY_LEN` bytes of memory where the key is read from. The size depends on the used algorithm, see above.
+
+// @return The function returns `EverCrypt_Error_Success` on success or
+//   `EverCrypt_Error_UnsupportedAlgorithm` in case of a bad algorithm identifier.
+//   (See `EverCrypt_Error.h`.)
+// */
+// EverCrypt_Error_error_code
+// EverCrypt_AEAD_create_in(Spec_Agile_AEAD_alg a, EverCrypt_AEAD_state_s **dst, uint8_t *k);
+
+val state_s : Type0
+
+val state_inv (s:NullableRef.ref state_s)
+              (k_bytes:bytes)
+  : vprop
+
+val dup_state_inv (#o:_)
+                  (s:NullableRef.ref state_s)
+                  (k:bytes)
+  : STGhostT unit o
+    (state_inv s k)
+    (fun _ -> state_inv s k `star` state_inv s k)
+    
+let maybe_vprop (b:bool) (p:vprop) = if b then p else emp
+
+val create_in (#a:_ { a == 0uy (* Spec.Agile.AEAD.AES128_GCM *) })
+              (dst:StRef.ref (NullableRef.ref state_s))
+              (#k_bytes:ebytes { Seq.length k_bytes == key_size })
+              (#k_p:perm)
+              (k:A.array U8.t)
+  : STT error_code
+        (A.pts_to k k_p k_bytes `star`
+         exists_ (StRef.pts_to dst full_perm))
+        (fun err ->
+          A.pts_to k k_p k_bytes `star`
+          exists_ (fun s_ptr -> 
+            StRef.pts_to dst full_perm s_ptr `star`
+            maybe_vprop (err = 0uy) (state_inv s_ptr k_bytes)))
+          
+
+// /**
+// Encrypt and authenticate a message (`plain`) with associated data (`ad`).
+
+// @param s Pointer to the The AEAD state created by `EverCrypt_AEAD_create_in`. It already contains the encryption key.
+// @param iv Pointer to `iv_len` bytes of memory where the nonce is read from.
+// @param iv_len Length of the nonce. Note: ChaCha20Poly1305 requires a 12 byte nonce.
+// @param ad Pointer to `ad_len` bytes of memory where the associated data is read from.
+// @param ad_len Length of the associated data.
+// @param plain Pointer to `plain_len` bytes of memory where the to-be-encrypted plaintext is read from.
+// @param plain_len Length of the to-be-encrypted plaintext.
+// @param cipher Pointer to `plain_len` bytes of memory where the ciphertext is written to.
+// @param tag Pointer to `TAG_LEN` bytes of memory where the tag is written to.
+//   The length of the `tag` must be of a suitable length for the chosen algorithm:
+//   * `Spec_Agile_AEAD_AES128_GCM` (TAG_LEN=16)
+//   * `Spec_Agile_AEAD_AES256_GCM` (TAG_LEN=16)
+//   * `Spec_Agile_AEAD_CHACHA20_POLY1305` (TAG_LEN=16)
+
+// @return `EverCrypt_AEAD_encrypt` may return either `EverCrypt_Error_Success` or `EverCrypt_Error_InvalidKey` (`EverCrypt_error.h`). The latter is returned if and only if the `s` parameter is `NULL`.
+// */
+// EverCrypt_Error_error_code
+// EverCrypt_AEAD_encrypt(
+//   EverCrypt_AEAD_state_s *s,
+//   uint8_t *iv,
+//   uint32_t iv_len,
+//   uint8_t *ad,
+//   uint32_t ad_len,
+//   uint8_t *plain,
+//   uint32_t plain_len,
+//   uint8_t *cipher,
+//   uint8_t *tag
+// );
+
+
+val encrypt (#k_bytes:ebytes { Seq.length k_bytes == key_size })
+            (s:NullableRef.ref state_s)
+            (#iv_p:perm)
+            (#iv_bytes:ebytes { Seq.length iv_bytes == iv_size })
+            (iv:A.array U8.t)
+            (iv_len:U32.t { U32.v iv_len == iv_size } )
+            (#in_p:perm)
+            (#in_bytes:ebytes)
+            (input:A.array U8.t)
+            (input_len:U32.t { A.length input == U32.v input_len /\
+                               U32.v input_len <= max_input_length /\ 
+                               Seq.length in_bytes == U32.v input_len })
+            (plain_unused:NullableRef.ref U8.t { plain_unused == NullableRef.null }) (* We're not using plain *)
+            (plain_len:U32.t { plain_len = 0ul })
+            (cipher_unused:NullableRef.ref U8.t { cipher_unused == NullableRef.null }) (* We're not using cipher *)
+            (tag:A.array U8.t { A.length tag == 16 })
+  : STT error_code
+    (requires
+       state_inv s k_bytes `star`
+       A.pts_to iv iv_p iv_bytes `star`
+       A.pts_to input in_p in_bytes `star`
+       exists_ (A.pts_to tag full_perm))
+    (ensures fun res ->
+       state_inv s k_bytes `star`
+       A.pts_to iv iv_p iv_bytes `star`
+       A.pts_to input in_p in_bytes `star`
+       exists_ (fun out ->
+         A.pts_to tag full_perm out `star`
+         pure (res == 0uy ==>  out == spec k_bytes iv_bytes in_bytes)))
+
+
+(** THE NO CHECK INTERFACE **)
+
 (* This is the C interface that we're trying to call from Steel 
 
   EverCrypt_Error_error_code
@@ -65,9 +183,9 @@ val encrypt_expand_aes128_gcm_no_check
       (input_len:U32.t { A.length input == U32.v input_len /\
                          U32.v input_len <= max_input_length /\ 
                          Seq.length in_bytes == U32.v input_len })
-      (plain_unused:R.ref U8.t { plain_unused == R.null }) (* We're not using plain *)
+      (plain_unused:NullableRef.ref U8.t { plain_unused == NullableRef.null }) (* We're not using plain *)
       (plain_len:U32.t { plain_len = 0ul })
-      (cipher_unused:R.ref U8.t { cipher_unused == R.null }) (* We're not using cipher *)
+      (cipher_unused:NullableRef.ref U8.t { cipher_unused == NullableRef.null }) (* We're not using cipher *)
       (tag:A.array U8.t { A.length tag == 16 })
   : STT error_code
     (requires
