steel/Zeta.Steel.AEADHandle.fst
@@ -1,0 +1,79 @@
+module Zeta.Steel.AEADHandle
+module G = Zeta.Steel.Globals
+module AEAD = EverCrypt.AEAD
+module R = Steel.ST.Reference
+module A = Steel.ST.Array
+module NullableRef = Steel.Reference
+open Steel.ST.Util
+
+let get_aead_key (_:unit)
+  : STGhostT perm Set.empty
+      emp
+      (fun p -> A.pts_to G.aead_key_buffer p G.aead_key)
+  =  let open G in
+     let body (_:unit)
+       : STGhostT perm (add_inv Set.empty aead_key_inv)
+           (exists_ (fun p -> A.pts_to aead_key_buffer p aead_key) `star` emp)
+           (fun q -> exists_ (fun p -> A.pts_to aead_key_buffer p aead_key) `star` 
+                  A.pts_to aead_key_buffer q aead_key)
+       = let p = elim_exists () in
+         A.share G.aead_key_buffer p (half_perm p) (half_perm p);
+         intro_exists (half_perm p) (fun p -> A.pts_to aead_key_buffer p aead_key);
+         half_perm p
+     in
+     with_invariant_g aead_key_inv body
+
+
+noeq
+type aead_handle_t = {
+   aead_state : NullableRef.ref AEAD.state_s;
+   aead_state_inv : inv (AEAD.state_inv aead_state G.aead_key)
+}
+
+let init_aead_handle () 
+  : STT aead_handle_t emp (fun _ -> emp)
+  = R.with_local #(NullableRef.ref AEAD.state_s) NullableRef.null (fun dst ->
+       assert_ (R.pts_to dst full_perm NullableRef.null);
+       let p = get_aead_key () in
+       let err = AEAD.create_in #0uy dst G.aead_key_buffer in
+       drop (A.pts_to G.aead_key_buffer _ _);       
+       let _st = elim_exists () in
+       let st = R.read dst in
+       intro_exists_erased _st (R.pts_to dst full_perm);       
+       if err = 0uy
+       then (
+         rewrite (AEAD.maybe_vprop _ _)
+                 (AEAD.state_inv st G.aead_key);
+         let inv = new_invariant (AEAD.state_inv st G.aead_key) in
+         let hdl = {
+             aead_state = st;
+             aead_state_inv = inv
+         } in
+         return hdl
+       )
+       else (
+         rewrite (AEAD.maybe_vprop _ _) emp;
+         let _ = G.abort "Failed AEAD initialization" in
+         return (false_elim ())
+       )
+    )
+    
+
+#push-options "--warn_error '-272'" //intentional top-level effect
+let aead_handle : aead_handle_t = init_aead_handle ()
+#pop-options
+
+let get_aead_state (_:unit)
+  : STT (NullableRef.ref AEAD.state_s)
+        emp
+        (fun p -> AEAD.state_inv p G.aead_key)
+  =  let body (_:unit)
+       : STGhostT unit
+                  (add_inv Set.empty aead_handle.aead_state_inv)
+                  (AEAD.state_inv aead_handle.aead_state G.aead_key `star` emp)
+                  (fun _ -> AEAD.state_inv aead_handle.aead_state G.aead_key `star`
+                         AEAD.state_inv aead_handle.aead_state G.aead_key)
+       = AEAD.dup_state_inv _ _
+     in
+     with_invariant_g aead_handle.aead_state_inv body;
+     return aead_handle.aead_state
