steel/Zeta.Steel.AEADHandle.fsti
@@ -1,0 +1,10 @@
+module Zeta.Steel.AEADHandle
+module G = Zeta.Steel.Globals
+module AEAD = EverCrypt.AEAD
+module NullableRef = Steel.Reference
+open Steel.ST.Util
+
+val get_aead_state (_:unit)
+  : STT (NullableRef.ref AEAD.state_s)
+        emp
+        (fun p -> AEAD.state_inv p G.aead_key)
