steel/Zeta.Steel.Globals.fsti
@@ -1,6 +1,7 @@
 module Zeta.Steel.Globals
 open Steel.ST.Util
 module A = Steel.ST.Array
+module R = Steel.ST.Reference
 module U8 = FStar.UInt8
 
 let aead_key_len = 16
@@ -10,3 +11,5 @@ let aead_key_buffer_t = k:A.array U8.t { A.length k == aead_key_len }
 val aead_key : k:Ghost.erased (Seq.seq U8.t) { Seq.length k == aead_key_len }
 val aead_key_buffer : aead_key_buffer_t
 val aead_key_inv : inv (exists_ (fun p -> A.pts_to aead_key_buffer p aead_key))
+
+val abort (msg:string) : STT (squash false) emp (fun _ -> emp)
